IsTrans, IsRefl, etc...

Foundation/Modal/Axioms.lean
@@ -80,9 +80,4 @@ protected abbrev L := □(□φ ➝ φ) ➝ □φ
 
 protected abbrev H := □(□φ ⭤ φ) ➝ □φ
 
-/--
-  Axiom for Geach confluency.
--/
-protected abbrev Geach (t : Geachean.Taple) (φ : F) := ◇^[t.i](□^[t.m]φ) ➝ □^[t.j](◇^[t.n]φ)
-
 end LO.Axioms
