Foundation/Modal/Kripke/AxiomGeach.lean
@@ -1,8 +1,59 @@
 import Foundation.Modal.Kripke.Completeness
 
-namespace LO.Modal
+namespace LO
+
+
+section
+
+variable {S F : Type*} [BasicModalLogicalConnective F] [Entailment F S]
+variable {𝓢 : S}
+
+/--
+  Axiom for Geach confluency.
+-/
+protected abbrev Axioms.Geach (g : Geachean.Taple) (φ : F) := ◇^[g.i](□^[g.m]φ) ➝ □^[g.j](◇^[g.n]φ)
+
+namespace Entailment
+
+class HasAxiomGeach (g) (𝓢 : S) where Geach (φ : F) : 𝓢 ⊢ Axioms.Geach g φ
+
+variable {g} [HasAxiomGeach g 𝓢]
+
+def axiomGeach : 𝓢 ⊢ ◇^[g.i](□^[g.m]φ) ➝ □^[g.j](◇^[g.n]φ) := HasAxiomGeach.Geach _
+@[simp] lemma axiomGeach! : 𝓢 ⊢! ◇^[g.i](□^[g.m]φ) ➝ □^[g.j](◇^[g.n]φ) := ⟨axiomGeach⟩
+
+instance [Entailment.HasAxiomT 𝓢] : Entailment.HasAxiomGeach ⟨0, 0, 1, 0⟩ 𝓢 := ⟨fun _ => axiomT⟩
+instance [Entailment.HasAxiomB 𝓢] : Entailment.HasAxiomGeach ⟨0, 1, 0, 1⟩ 𝓢 := ⟨fun _ => axiomB⟩
+instance [Entailment.HasAxiomD 𝓢] : Entailment.HasAxiomGeach ⟨0, 0, 1, 1⟩ 𝓢 := ⟨fun _ => axiomD⟩
+instance [Entailment.HasAxiomFour 𝓢] : Entailment.HasAxiomGeach ⟨0, 2, 1, 0⟩ 𝓢 := ⟨fun _ => axiomFour⟩
+instance [Entailment.HasAxiomFive 𝓢] : Entailment.HasAxiomGeach ⟨1, 1, 0, 1⟩ 𝓢 := ⟨fun _ => axiomFive⟩
+instance [Entailment.HasAxiomTc 𝓢] : Entailment.HasAxiomGeach ⟨0, 1, 0, 0⟩ 𝓢 := ⟨fun _ => axiomTc⟩
+instance [Entailment.HasAxiomPoint2 𝓢] : Entailment.HasAxiomGeach ⟨1, 1, 1, 1⟩ 𝓢 := ⟨fun _ => axiomPoint2⟩
+
+end Entailment
+
+end
+
+
+namespace Modal
 
 namespace Kripke
+
+instance whitepoint.instIsGeachean : IsGeachean g _ whitepoint.Rel := ⟨by
+  rintro x y z ⟨Rxy, Rxz⟩;
+  use ();
+  constructor;
+  . apply Rel.iterate.true_any; tauto;
+  . apply Rel.iterate.true_any; tauto;
+⟩
+
+instance : IsRefl _ whitepoint.Rel := by
+  have := whitepoint.instIsGeachean (g := ⟨0, 0, 1, 0⟩);
+  infer_instance;
+
+instance : IsTrans _ whitepoint.Rel := by
+  have := whitepoint.instIsGeachean (g := ⟨0, 2, 1, 0⟩);
+  infer_instance;
 
 open Formula.Kripke
 
@@ -13,21 +64,27 @@ section definability
 
 variable {F : Kripke.Frame} {g : Geachean.Taple}
 
-lemma validate_AxiomGeach_of_Geachean (hG : (Geachean g) F.Rel) : F ⊧ (Axioms.Geach g (.atom 0)) := by
+lemma validate_AxiomGeach_of_Geachean [IsGeachean g _ F.Rel] : F ⊧ (Axioms.Geach g (.atom 0)) := by
   rintro V x h;
   apply Satisfies.multibox_def.mpr;
   obtain ⟨y, Rxy, hbp⟩ := Satisfies.multidia_def.mp h;
   intro z Rxz;
   apply Satisfies.multidia_def.mpr;
-  obtain ⟨u, Ryu, Rzu⟩ := hG ⟨Rxy, Rxz⟩;
+  obtain ⟨u, Ryu, Rzu⟩ := IsGeachean.geachean ⟨Rxy, Rxz⟩;
   use u;
   constructor;
   . assumption;
   . exact (Satisfies.multibox_def.mp hbp) Ryu;
 
-
 section
 
+lemma validate_AxiomT_of_reflexive [refl : IsRefl _ F] : F ⊧ (Axioms.T (.atom 0)) := by
+  exact validate_AxiomGeach_of_Geachean (g := ⟨0, 0, 1, 0⟩);
+
+lemma validate_AxiomFour_of_transitive [trans : IsTrans _ F] : F ⊧ (Axioms.Four (.atom 0)) := by
+  exact validate_AxiomGeach_of_Geachean (g := ⟨0, 2, 1, 0⟩);
+
+/-
 lemma validate_AxiomT_of_reflexive (h : Reflexive F.Rel) : F ⊧ (Axioms.T (.atom 0)) := by
   rw [Geachean.reflexive_def] at h;
   exact validate_AxiomGeach_of_Geachean h;
@@ -55,6 +112,7 @@ lemma validate_AxiomPoint2_of_confluent (h : Confluent F.Rel) : F ⊧ (Axioms.Po
 lemma validate_AxiomTc_of_coreflexive (h : Coreflexive F.Rel) : F ⊧ (Axioms.Tc (.atom 0)) := by
   rw [Geachean.coreflexive_def] at h;
   exact validate_AxiomGeach_of_Geachean h;
+-/
 
 end
 
@@ -147,9 +205,7 @@ open canonicalModel
 
 namespace Canonical
 
-protected lemma geachean
-  (hG : ∀ {φ}, 𝓢 ⊢! ◇^[g.i](□^[g.m]φ) ➝ □^[g.j](◇^[g.n]φ))
-  : Geachean g (canonicalFrame 𝓢).Rel := by
+protected lemma geachean [Entailment.HasAxiomGeach g 𝓢] : IsGeachean g _ (canonicalFrame 𝓢).Rel := ⟨by
   rintro x y z ⟨Rxy, Rxz⟩;
   have ⟨u, hu⟩ := lindenbaum (𝓢 := 𝓢) (t₀ := ⟨□''⁻¹^[g.m]y.1.1, ◇''⁻¹^[g.n]z.1.2⟩) $ by
     rintro Γ Δ hΓ hΔ;
@@ -172,7 +228,7 @@ protected lemma geachean
     have : 𝓢 ⊢! □^[g.m]γ ➝ □^[g.m]δ := imply_multibox_distribute'! hC;
     have : □^[g.m]δ ∈ y.1.1 := mdp_mem₁_provable this hγ;
     have : ◇^[g.i](□^[g.m]δ) ∈ x.1.1 := def_multirel_multidia_mem₁.mp Rxy this;
-    have : □^[g.j](◇^[g.n]δ) ∈ x.1.1 := mdp_mem₁_provable hG this;
+    have : □^[g.j](◇^[g.n]δ) ∈ x.1.1 := mdp_mem₁_provable axiomGeach! this;
     have : ◇^[g.n]δ ∈ z.1.1 := def_multirel_multibox_mem₁.mp Rxz this;
     have : ◇^[g.n]δ ∉ z.1.2 := iff_not_mem₂_mem₁.mpr this;
     contradiction;
@@ -184,10 +240,28 @@ protected lemma geachean
   . apply def_multirel_multidia_mem₂.mpr;
     intro φ hφ;
     exact hu.2 hφ;
+⟩
 
-protected lemma reflexive [Entailment.HasAxiomT 𝓢] : Reflexive (canonicalFrame 𝓢).Rel := by
-  rw [Geachean.reflexive_def]; apply Canonical.geachean; simp [axiomT!];
+protected lemma transitive [Entailment.HasAxiomFour 𝓢] : IsTrans _ (canonicalFrame 𝓢).Rel := by
+  have := Canonical.geachean (𝓢 := 𝓢) (g := ⟨0, 2, 1, 0⟩);
+  infer_instance;
 
+protected lemma reflexive [Entailment.HasAxiomT 𝓢] : IsRefl _ (canonicalFrame 𝓢).Rel := by
+  have := Canonical.geachean (𝓢 := 𝓢) (g := ⟨0, 0, 1, 0⟩);
+  infer_instance;
+
+
+/-
+protected lemma reflexive [Entailment.HasAxiomT 𝓢] : IsRefl _ (canonicalFrame 𝓢).Rel := ⟨by
+  have := @Canonical.geachean (g := ⟨0, 0, 1, 0⟩);
+  rw [←Geachean.reflexive_def] at this;
+  apply Canonical.geachean;
+  intro x;
+  simp [axiomT!];
+⟩
+-/
+
+/-
 protected lemma transitive [Entailment.HasAxiomFour 𝓢] : Transitive (canonicalFrame 𝓢).Rel := by
   rw [Geachean.transitive_def]; apply Canonical.geachean; simp [axiomFour!];
 
@@ -205,6 +279,7 @@ protected lemma coreflexive [Entailment.HasAxiomTc 𝓢] : Coreflexive (canonica
 
 protected lemma confluent [Entailment.HasAxiomPoint2 𝓢] : Confluent (canonicalFrame 𝓢).Rel := by
   rw [Geachean.confluent_def]; apply Canonical.geachean; simp [axiomPoint2!];
+-/
 
 end Canonical
 
