Foundation/Modal/Kripke/Hilbert/Geach.lean
@@ -1,32 +1,92 @@
-import Foundation.Modal.Hilbert.Geach
 import Foundation.Modal.Kripke.AxiomGeach
 import Foundation.Modal.Kripke.Hilbert.Soundness
+import Foundation.Modal.Hilbert.WellKnown
 
 namespace LO.Modal
 
-open Formula.Kripke
-
 /-
-namespace Kripke
+namespace Hilbert
 
-instance FrameClass.multiGeachean.definability' (G)
-  : (FrameClass.multiGeachean G).DefinedBy (Hilbert.Geach G).axioms :=
-  FrameClass.definedBy_with_axiomK (FrameClass.multiGeachean.definability G)
+variable (α) [DecidableEq α]
 
-end Kripke
+protected abbrev Geach (G : Set (Geachean.Taple)) : Hilbert ℕ := ⟨
+  {Axioms.K (.atom 0) (.atom 1)}
+  ∪ G.image (λ t => Axioms.Geach t (.atom 0))
+⟩
+
+instance : HasK (Hilbert.Geach G) where p := 0; q := 1
+instance : Entailment.K (Hilbert.Geach G) where
+
+lemma K4.eq_Geach     : Hilbert.K4     = Hilbert.Geach {⟨0, 2, 1, 0⟩} := by aesop;
+lemma K45.eq_Geach    : Hilbert.K45    = Hilbert.Geach {⟨0, 2, 1, 0⟩, ⟨1, 1, 0, 1⟩} := by aesop;
+lemma K5.eq_Geach     : Hilbert.K5     = Hilbert.Geach {⟨1, 1, 0, 1⟩} := by aesop;
+lemma KB.eq_Geach     : Hilbert.KB     = Hilbert.Geach {⟨0, 1, 0, 1⟩} := by aesop;
+lemma KB4.eq_Geach    : Hilbert.KB4    = Hilbert.Geach {⟨0, 1, 0, 1⟩, ⟨0, 2, 1, 0⟩} := by aesop;
+lemma KB5.eq_Geach    : Hilbert.KB5    = Hilbert.Geach {⟨0, 1, 0, 1⟩, ⟨1, 1, 0, 1⟩} := by aesop;
+lemma KD.eq_Geach     : Hilbert.KD     = Hilbert.Geach {⟨0, 0, 1, 1⟩} := by aesop;
+lemma KD4.eq_Geach    : Hilbert.KD4    = Hilbert.Geach {⟨0, 0, 1, 1⟩, ⟨0, 2, 1, 0⟩} := by aesop;
+lemma KD45.eq_Geach   : Hilbert.KD45   = Hilbert.Geach {⟨0, 0, 1, 1⟩, ⟨0, 2, 1, 0⟩, ⟨1, 1, 0, 1⟩} := by aesop;
+lemma KD5.eq_Geach    : Hilbert.KD5    = Hilbert.Geach {⟨0, 0, 1, 1⟩, ⟨1, 1, 0, 1⟩} := by aesop;
+lemma KDB.eq_Geach    : Hilbert.KDB    = Hilbert.Geach {⟨0, 0, 1, 1⟩, ⟨0, 1, 0, 1⟩} := by aesop;
+lemma KT.eq_Geach     : Hilbert.KT     = Hilbert.Geach {⟨0, 0, 1, 0⟩} := by aesop;
+lemma KT4B.eq_Geach   : Hilbert.KT4B   = Hilbert.Geach {⟨0, 0, 1, 0⟩, ⟨0, 2, 1, 0⟩, ⟨0, 1, 0, 1⟩} := by aesop;
+lemma KTB.eq_Geach    : Hilbert.KTB    = Hilbert.Geach {⟨0, 0, 1, 0⟩, ⟨0, 1, 0, 1⟩} := by aesop;
+lemma KTc.eq_Geach    : Hilbert.KTc    = Hilbert.Geach {⟨0, 1, 0, 0⟩} := by aesop;
+lemma S4.eq_Geach     : Hilbert.S4     = Hilbert.Geach {⟨0, 0, 1, 0⟩, ⟨0, 2, 1, 0⟩} := by aesop;
+lemma S4Point2.eq_Geach : Hilbert.S4Point2 = Hilbert.Geach {⟨0, 0, 1, 0⟩, ⟨0, 2, 1, 0⟩, ⟨1, 1, 1, 1⟩} := by aesop;
+lemma S5.eq_Geach     : Hilbert.S5     = Hilbert.Geach {⟨0, 0, 1, 0⟩, ⟨1, 1, 0, 1⟩} := by aesop;
+lemma Triv.eq_Geach   : Hilbert.Triv   = Hilbert.Geach {⟨0, 0, 1, 0⟩, ⟨0, 1, 0, 0⟩} := by aesop;
+
+instance HasT_of_mem_0_0_1_0 (h : ⟨0, 0, 1, 0⟩ ∈ G) : HasT (Hilbert.Geach G) where
+  p := 0
+  mem_T := by
+    simp [Hilbert.Geach];
+    use ⟨0, 0, 1, 0⟩;
+    simpa;
+
+instance HasB_of_mem_0_1_0_1 (h : ⟨0, 1, 0, 1⟩ ∈ G) : HasB (Hilbert.Geach G) where
+  p := 0
+  mem_B := by
+    simp [Hilbert.Geach];
+    use ⟨0, 1, 0, 1⟩;
+    simpa;
+
+instance HasD_of_mem_0_0_1_1 (h : ⟨0, 0, 1, 1⟩ ∈ G) : HasD (Hilbert.Geach G) where
+  p := 0
+  mem_D := by
+    simp [Hilbert.Geach];
+    use ⟨0, 0, 1, 1⟩;
+    simpa;
+
+instance HasFour_of_mem_0_2_1_0 (h : ⟨0, 2, 1, 0⟩ ∈ G) : HasFour (Hilbert.Geach G) where
+  p := 0
+  mem_Four := by
+    simp [Hilbert.Geach];
+    use ⟨0, 2, 1, 0⟩;
+    simpa;
+
+instance HasFive_of_mem_1_1_0_1 (h : ⟨1, 1, 0, 1⟩ ∈ G) : HasFive (Hilbert.Geach G) where
+  p := 0
+  mem_Five := by
+    simp [Hilbert.Geach];
+    use ⟨1, 1, 0, 1⟩;
+    simpa;
+
+instance HasPoint2_of_mem_1_1_1_1 (h : ⟨1, 1, 1, 1⟩ ∈ G) : HasPoint2 (Hilbert.Geach G) where
+  p := 0
+  mem_Point2 := by
+    simp [Hilbert.Geach];
+    use ⟨1, 1, 1, 1⟩;
+    simpa;
+
+instance HasTc_of_mem_0_1_0_0 (h : ⟨0, 1, 0, 0⟩ ∈ G) : HasTc (Hilbert.Geach G) where
+  p := 0
+  mem_Tc := by
+    simp [Hilbert.Geach];
+    use ⟨0, 1, 0, 0⟩;
+    simpa;
+
+end Hilbert
 -/
-
-
-namespace Hilbert.Geach
-
-open Kripke
-open Hilbert.Kripke
-
--- instance Kripke.sound : Sound (Hilbert.Geach G) (FrameClass.multiGeachean G) := inferInstance
-
--- instance Kripke.consistent : Entailment.Consistent (Hilbert.Geach G) := consistent_of_sound (FrameClass.multiGeachean G) (by simp)
-
-end Hilbert.Geach
-
 
 end LO.Modal
